Enable proofs by reflection for InvokedBy* (bool based variants implemented) [skip ci]

theories/Program.v
@@ -40,6 +40,25 @@ Module Type ProgramMixin (B : Base)
   (Import FDecl : FunDecl B)
   (Import FDK : FunDefKit B FDecl).
 
+  Definition 𝑭_eqb {Δ1 Δ2 τ1 τ2} (f1 : 𝑭 Δ1 τ1) (f2 : 𝑭 Δ2 τ2) : bool :=
+    if @Classes.eq_dec _ 𝑭_eq_dec (existT _ (existT _ f1)) (existT _ (existT _ f2))
+    then true
+    else false.
+
+  (* TODO: very annoying definition, but otherwise the wrong eq with existT pops up,
+           see commented out definition below
+           (we get `existT (𝑭 Δ) ...` instead of `existT Δ ...`) *)
+  (* Definition wrong {Δ1 Δ2 τ1 τ2} (f1 : 𝑭 Δ1 τ1) (f2 : 𝑭 Δ2 τ2) : Prop :=
+    existT _ (existT _ f1) = existT _ (existT _ f2).
+  Print wrong. *)
+  Definition 𝑭_eq {Δ1 Δ2 τ1 τ2} (f1 : 𝑭 Δ1 τ1) (f2 : 𝑭 Δ2 τ2) : Prop :=
+   (@existT (NCtx (@PVar B.varkit) (@Ty B.typedeclkit))
+      (fun Γ : NCtx (@PVar B.varkit) (@Ty B.typedeclkit) => {x : @Ty B.typedeclkit & 𝑭 Γ x}) Δ1
+      (@existT (@Ty B.typedeclkit) (𝑭 Δ1) τ1 f1)) =
+   (@existT (NCtx (@PVar B.varkit) (@Ty B.typedeclkit))
+      (fun Γ : NCtx (@PVar B.varkit) (@Ty B.typedeclkit) => {x : @Ty B.typedeclkit & 𝑭 Γ x}) Δ2
+      (@existT (@Ty B.typedeclkit) (𝑭 Δ2) τ2 f2)).
+
   Section InvokedByStm.
     Variable invoke_call : forall {Δ τ1 τ2 Γ}, 𝑭 Δ τ1 -> Stm Γ τ2 -> Prop.
 
@@ -50,8 +69,7 @@ Module Type ProgramMixin (B : Base)
       | stm_let x σ s1 s2 => InvokedByStm_aux f s1 \/ InvokedByStm_aux f s2
       | stm_block δ s => InvokedByStm_aux f s
       | stm_assign xInΓ s => InvokedByStm_aux f s
-      | stm_call f2 es => existT _ (existT _ f) = existT _ (existT _ f2)
-                          \/ invoke_call f (FunDef f2)
+      | stm_call f2 es => 𝑭_eq f f2 \/ invoke_call f (FunDef f2)
       | stm_call_frame δ s => InvokedByStm_aux f s
       | stm_foreign f es => False
       | stm_lemmak l es k => InvokedByStm_aux f k
@@ -61,16 +79,49 @@ Module Type ProgramMixin (B : Base)
       | stm_pattern_match s pat rhs => InvokedByStm_aux f s \/ (exists pc, InvokedByStm_aux f (rhs pc))
       | stm_read_register reg => False
       | stm_write_register reg e => False
-      | stm_bind s k => InvokedByStm_aux f s \/ (exists v, InvokedByStm_aux f (k v))
+      | stm_bind s k => False (* stm_bind should not be used in source code directly, hence we don't include it in the search of fn invocations *)
       | stm_debugk k => InvokedByStm_aux f k
       end.
   End InvokedByStm.
 
+  Section InvokedByStmBool.
+    Variable invoke_call : forall {Δ τ1 τ2 Γ}, 𝑭 Δ τ1 -> Stm Γ τ2 -> bool.
+
+    Fixpoint InvokedByStmB_aux {Δ τ1 τ2 Γ} (f : 𝑭 Δ τ1) (s : Stm Γ τ2) : bool :=
+      match s with
+      | stm_val _ v => false
+      | stm_exp e => false
+      | stm_let x σ s1 s2 => InvokedByStmB_aux f s1 || InvokedByStmB_aux f s2
+      | stm_block δ s => InvokedByStmB_aux f s
+      | stm_assign xInΓ s => InvokedByStmB_aux f s
+      | stm_call f2 es => 𝑭_eqb f f2 || invoke_call f (FunDef f2)
+      | stm_call_frame δ s => InvokedByStmB_aux f s
+      | stm_foreign f es => false
+      | stm_lemmak l es k => InvokedByStmB_aux f k
+      | stm_seq s k => InvokedByStmB_aux f s || InvokedByStmB_aux f k
+      | stm_assertk e1 e2 k => InvokedByStmB_aux f k
+      | stm_fail _ s => false
+      | stm_pattern_match s pat rhs =>
+          InvokedByStmB_aux f s
+          || List.existsb (fun pc => InvokedByStmB_aux f (rhs pc))
+                          (@finite.enum _ _ (B.Finite_PatternCase pat))
+      | stm_read_register reg => false
+      | stm_write_register reg e => false
+      | stm_bind s k => false
+      | stm_debugk k => InvokedByStmB_aux f k
+      end.
+  End InvokedByStmBool.
+
   Fixpoint InvokedByStmWithFuel (fuel : nat) {Δ τ1 τ2 Γ} (f : 𝑭 Δ τ1) (s : Stm Γ τ2) : Prop :=
     match fuel with
-    (* | 0 => False *)
     | 0 => InvokedByStm_aux (fun _ _ _ _ _ _ => False) f s
     | S fuel => InvokedByStm_aux (@InvokedByStmWithFuel fuel) f s
+    end.
+
+  Fixpoint InvokedByStmWithFuelBool (fuel : nat) {Δ τ1 τ2 Γ} (f : 𝑭 Δ τ1) (s : Stm Γ τ2) : bool :=
+    match fuel with
+    | 0 => InvokedByStmB_aux (fun _ _ _ _ _ _ => false) f s
+    | S fuel => InvokedByStmB_aux (@InvokedByStmWithFuelBool fuel) f s
     end.
 
   Lemma InvokedByStmWithFuel_S_fuel : forall (fuel : nat) {Δ τ1 τ2 Γ} (f : 𝑭 Δ τ1) (s : Stm Γ τ2),
@@ -91,10 +142,6 @@ Module Type ProgramMixin (B : Base)
         * left. now apply IHs.
         * right. destruct Hinvok as [pc Hinvok].
           exists pc. now apply H.
-      + destruct Hinvok as [Hinvok|Hinvok].
-        * left. now apply IHs.
-        * right. destruct Hinvok as [v Hinvok].
-          exists v. now apply H.
     - induction s; cbn in *; auto.
       + destruct Hinvok.
         * left. now apply IHs1.
@@ -107,20 +154,21 @@ Module Type ProgramMixin (B : Base)
         * left. now apply IHs.
         * right. destruct Hinvok as [pc Hinvok].
           exists pc. now apply H.
-      + destruct Hinvok as [Hinvok|Hinvok].
-        * left. now apply IHs.
-        * right. destruct Hinvok as [v Hinvok].
-          exists v. now apply H.
   Qed.
 
   Definition InvokedByStm {Δ τ1 τ2 Γ} (f : 𝑭 Δ τ1) (s : Stm Γ τ2) : Prop :=
     InvokedByStmWithFuel 2 f s.
 
-  Definition InvokedByFun (fuel : nat) {Δ1 τ1} {Δ2 τ2} (f1 : 𝑭 Δ1 τ1) (f2 : 𝑭 Δ2 τ2) :=
-    (* existT _ (existT _ f1) <> existT _ (existT _ f2) /\ *)
+  Definition InvokedByStmBool {Δ τ1 τ2 Γ} (f : 𝑭 Δ τ1) (s : Stm Γ τ2) : bool :=
+    InvokedByStmWithFuelBool 2 f s.
+
+  Definition InvokedByFun (fuel : nat) {Δ1 τ1} {Δ2 τ2} (f1 : 𝑭 Δ1 τ1) (f2 : 𝑭 Δ2 τ2) : Prop :=
     InvokedByStmWithFuel fuel f1 (FunDef f2).
 
-  Definition InvokedByFun_S_fuel : forall (fuel : nat) {Δ1 τ1} {Δ2 τ2} (f1 : 𝑭 Δ1 τ1) (f2 : 𝑭 Δ2 τ2),
+  Definition InvokedByFunBool (fuel : nat) {Δ1 τ1} {Δ2 τ2} (f1 : 𝑭 Δ1 τ1) (f2 : 𝑭 Δ2 τ2) : bool :=
+    InvokedByStmWithFuelBool fuel f1 (FunDef f2).
+
+  Lemma InvokedByFun_S_fuel : forall (fuel : nat) {Δ1 τ1} {Δ2 τ2} (f1 : 𝑭 Δ1 τ1) (f2 : 𝑭 Δ2 τ2),
     InvokedByFun fuel f1 f2 ->
     InvokedByFun (S fuel) f1 f2.
   Proof.
@@ -129,9 +177,14 @@ Module Type ProgramMixin (B : Base)
     apply InvokedByStmWithFuel_S_fuel.
   Qed.
 
-  Definition InvokedByFunPackage (fuel : nat) (f1 f2 : {Δ & {τ & 𝑭 Δ τ}}) :=
+  Definition InvokedByFunPackage (fuel : nat) (f1 f2 : {Δ & {τ & 𝑭 Δ τ}}) : Prop :=
     match f1, f2 with
     | existT Δ1 (existT τ1 f1) ,  existT Δ2 (existT τ2 f2) => InvokedByFun fuel f1 f2
+    end.
+
+  Definition InvokedByFunPackageBool (fuel : nat) (f1 f2 : {Δ & {τ & 𝑭 Δ τ}}) : bool :=
+    match f1, f2 with
+    | existT Δ1 (existT τ1 f1) ,  existT Δ2 (existT τ2 f2) => InvokedByFunBool fuel f1 f2
     end.
 
   Lemma InvokedByFunPackage_S_fuel : forall (fuel : nat) (f1 f2 : {Δ & {τ & 𝑭 Δ τ}}),
@@ -152,6 +205,76 @@ Module Type ProgramMixin (B : Base)
     intros [Δ1 [τ1 f1]] [Δ2 [τ2 f2]] Hinvok.
     now apply InvokedByFunPackage_S_fuel.
   Qed.
+
+  Section InvokedByReflect.
+    Lemma InvokedByStmWithFuel_spec : forall {Δ τ1 τ2 Γ} (fuel : nat) (f : 𝑭 Δ τ1) (s : Stm Γ τ2),
+      Bool.reflect (InvokedByStmWithFuel fuel f s) (InvokedByStmWithFuelBool fuel f s).
+    Proof.
+      intros Δ τ1 τ2 Γ fuel f s.
+      apply Bool.iff_reflect. split; intros H.
+      - generalize dependent s.
+        generalize dependent f.
+        generalize dependent Γ.
+        generalize dependent τ2.
+        generalize dependent τ1.
+        generalize dependent Δ.
+        induction fuel; intros Δ τ1 τ2 Γ f s H.
+        + induction s; cbn in *; auto.
+          * apply Bool.orb_true_iff; destruct H as [H|H]; auto.
+          * destruct H as [H|?]; auto.
+            apply Bool.orb_true_iff. left.
+            unfold 𝑭_eq in H. unfold 𝑭_eqb.
+            destruct (Classes.eq_dec _ _) eqn:E; auto.
+          * apply Bool.orb_true_iff; destruct H as [H|H]; auto.
+          * apply Bool.orb_true_iff; destruct H as [H|[pc H]]; auto.
+            right. clear IHs.
+            apply List.existsb_exists. exists pc. split; auto.
+            apply base.elem_of_list_In.
+            apply finite.elem_of_enum.
+        + induction s; cbn in *; auto.
+          * apply Bool.orb_true_iff; destruct H as [H|H]; auto.
+          * apply Bool.orb_true_iff; destruct H as [H|H]; auto.
+            left. unfold 𝑭_eq in H. unfold 𝑭_eqb.
+            destruct (Classes.eq_dec _ _) eqn:E; auto.
+          * apply Bool.orb_true_iff; destruct H as [H|H]; auto.
+          * apply Bool.orb_true_iff; destruct H as [H|[pc H]]; auto.
+            right. clear IHs.
+            apply List.existsb_exists. exists pc. split; auto.
+            apply base.elem_of_list_In.
+            apply finite.elem_of_enum.
+      - generalize dependent s.
+        generalize dependent f.
+        generalize dependent Γ.
+        generalize dependent τ2.
+        generalize dependent τ1.
+        generalize dependent Δ.
+        induction fuel; intros Δ τ1 τ2 Γ f s H.
+        + induction s; cbn in *; auto.
+          * apply Bool.orb_true_iff in H; destruct H; auto.
+          * apply Bool.orb_true_iff in H; destruct H; auto.
+            left. unfold 𝑭_eqb in H. unfold 𝑭_eq.
+            destruct (Classes.eq_dec _ _) eqn:E; auto; try discriminate.
+          * apply Bool.orb_true_iff in H; destruct H; auto.
+          * apply Bool.orb_true_iff in H; destruct H as [?|[pc [HIn H]]%List.existsb_exists]; auto.
+            clear IHs. right. exists pc. auto.
+        + induction s; cbn in *; auto.
+          * apply Bool.orb_true_iff in H; destruct H; auto.
+          * apply Bool.orb_true_iff in H; destruct H; auto.
+            left. unfold 𝑭_eqb in H. unfold 𝑭_eq.
+            destruct (Classes.eq_dec _ _) eqn:E; auto; try discriminate.
+          * apply Bool.orb_true_iff in H; destruct H; auto.
+          * apply Bool.orb_true_iff in H; destruct H as [?|[pc [HIn H]]%List.existsb_exists]; auto.
+            clear IHs. right. exists pc. auto.
+    Qed.
+
+    Lemma InvokedByFunPackage_spec : forall (fuel : nat) (f1 f2 : {Δ & {τ & 𝑭 Δ τ}}),
+      Bool.reflect (InvokedByFunPackage fuel f1 f2) (InvokedByFunPackageBool fuel f1 f2).
+    Proof.
+      unfold InvokedByFunPackage, InvokedByFun.
+      intros fuel [Δ1 [τ1 f1]] [Δ2 [τ2 f2]].
+      apply InvokedByStmWithFuel_spec.
+    Qed.
+  End InvokedByReflect.
 End ProgramMixin.
 
 Module Type WellFoundedKit (B : Base) (FDecl : FunDecl B) (FDK : FunDefKit B FDecl)
